AP/AP/Defense/Edge/WF.lean
@@ -3,8 +3,10 @@ import AP.AP.Defense.Edge.Symmetry
 namespace AP.Edge
 
 variable {e e₁ e₂ : Edge}
+variable {s : State} [hpw : Fact # s.pw = 1]
+omit hpw
 
-def cndAux₀ (s : State) : Prop :=
+def cnd₀ (s : State) : Prop :=
   let pa := s.aPos
   let p₀ := edge₀.getBorderPoint₀ pa
   let get := edge₀.getBorderPoints pa
@@ -16,69 +18,84 @@ def cndAux₀ (s : State) : Prop :=
   | 1 => (p₀ :: get 1).all (· ∈ s.taken)
   | d => 0 < d
 
-def cnd₀ (s : State) : Prop :=
-  if s.aTurn then cndAux₀ s else
-  ∃ s₀, cndAux₀ s₀ ∧ ∃ p, sys.tr s₀ p = some s
+theorem aPos_y_lt_zero_of_cnd₀ (h : cnd₀ s) : s.aPos.y < 0 := by
+  simp [cnd₀, getBorderPoints, getBorderPoint₀, getBorderPoint] at h ⊢
+  split at h <;> linarith
 
-theorem aPos_y_lt_zero_of_cnd₀ {s} (h : cnd₀ s) : s.aPos.y < 0 := by
-  -- cases ht : s.aTurn
-  -- · simp [cnd₀, ht] at h
-  --   choose s₀ h p h₁ using h
-  --   have h₂ := State.aTurn_eq_of_tr h₁
-  --   simp [ht] at h₂
-  --   simp [cnd₀, getBorderPoints, getBorderPoint₀, getBorderPoint, dist, ht] at h ⊢
-  --   split at h <;> linarith
-  -- · simp [cnd₀, cndAux₀, ht] at h; exact h
-  sorry
+theorem cnd₀_of_aPos_y_le_neg_6 (h : s.aPos.y ≤ -6) : cnd₀ s := by
+  simp [cnd₀, getBorderPoints, getBorderPoint₀, getBorderPoint] at h ⊢
+  split <;> linarith
 
--- #check 0 #exit
-
-theorem cnd₀_of_aPos_y_le_neg_6 {s} (h : s.aPos.y ≤ -6) : cnd₀ s := by
-  -- cases ht : s.aTurn
-  -- · simp [cnd₀, getBorderPoints, getBorderPoint₀, getBorderPoint, dist, ht] at h ⊢
-  --   split <;> linarith
-  -- · simp [cnd₀, ht]; linarith
-  sorry
-
-theorem cnd₀_simulatemul_two_full_of_aState {s s₁} {a : AStrat} {d : DStrat} {n}
+include hpw in
+theorem cnd₀_simulatemul_two_full_of_aState {s₁} {a : AStrat} {d : DStrat} {n}
 [hs : AState s] [ha : a.WF] [hd : d.WF] (h₁ : cnd₀ s)
-(h₂ : sys.simulate (Strat.f ⟨a, edge₀.defense.st d⟩) s (n * 2) = (s₁, 0)): cnd₀ s₁ := by
+(h₂ : sys.simulate (Strat.f ⟨a, edge₀.defense.st d⟩) s (n * 2) = (s₁, 0)) : cnd₀ s₁ := by
   induction n
   · sorry
   · sorry
 
-theorem cnd₀_of_aState_tr {s s' p} [hs : AState s]
-(h₁ : sys.tr s p = some s') (h₂ : cnd₀ s) : cnd₀ s' := by
-  -- have hs' := DState.of_tr h₁
-  -- simp [cnd₀] at h₂
-  -- simp [cnd₀, getBorderPoints, getBorderPoint₀, getBorderPoint, dist]
-  sorry
-
 -- #check 0 #exit
 
-theorem cnd₀_simulate_full_of_aState {s s₁} {a : AStrat} {d : DStrat} {n}
-[hs : AState s] [ha : a.WF] [hd : d.WF] (h₁ : cnd₀ s)
-(h₂ : sys.simulate (Strat.f ⟨a, edge₀.defense.st d⟩) s n = (s₁, 0)) : cnd₀ s₁ := by
+include hpw in
+theorem aPos_y_lt_zero_of_tr_aState_cnd₀ {s' p} [hs : AState s]
+(h₁ : cnd₀ s) (h₂ : sys.tr s p = some s') : s'.aPos.y < 0 := by
+  replace hpw := hpw.1
+  rw [hs.tr_eq_some_iff] at h₂
+  rcases h₂ with ⟨⟨h₂, h₃, h₄⟩, rfl⟩
+  dsimp
+  simp [Point.dist, hpw] at h₄
+  rcases h₄ with ⟨hx, h₄⟩
+  simp [abs_le] at h₄
+  rcases h₄ with ⟨-, h₄⟩
+  have h₅ := aPos_y_lt_zero_of_cnd₀ h₁
+  rw [lt_iff_le_and_ne]
+  split_ands; linarith
+  intro h₆
+  simp [h₆] at h₄
+  rw [add_comm, ←neg_le_iff_add_nonneg] at h₄
+  replace h₄ : s.aPos.y = -1; omega; clear h₅
+  clear hpw h₂
+  simp [cnd₀, h₄, getBorderPoints, getBorderPoint₀, getBorderPoint] at h₁
+  rcases h₁ with ⟨H₁, H₂, H₃⟩
+  apply h₃; clear h₃
+  replace hx : p.x ∈ (s.aPos.x + ·) '' {-1, 0, 1}
+  · simp; simp [abs_le] at hx; omega
+  simp at hx
+  rcases p with ⟨x, y⟩
+  dsimp at *
+  subst h₆
+  rcases hx with hx | hx | hx
+  · convert H₂; linarith
+  · convert H₁; linarith
+  · convert H₃; linarith
+
+include hpw in
+theorem edge₀_simulate_full_aPos_y_lt_zero_of_aState {s₁} {a : AStrat} {d : DStrat} {n}
+[hs : AState s] [ha : a.WF] [hd : d.WF] (h₁ : s.aPos.y ≤ -6)
+(h₂ : sys.simulate (Strat.f ⟨a, edge₀.defense.st d⟩) s n = (s₁, 0)) : s₁.aPos.y < 0 := by
+  have H := cnd₀_of_aPos_y_le_neg_6 h₁
   induction n using Nat.mod_2_ind <;> nm n
-  · exact cnd₀_simulatemul_two_full_of_aState h₁ h₂
+  · apply aPos_y_lt_zero_of_cnd₀
+    apply cnd₀_simulatemul_two_full_of_aState H h₂
   rw [sys.simulate_succ_full'] at h₂
   choose s' h₂ h₃ using h₂
-  have h₄ := cnd₀_simulatemul_two_full_of_aState h₁ h₂
+  have h₄ := cnd₀_simulatemul_two_full_of_aState H h₂
   have hs' := AState.of_simulate_mul_two_eq_full h₂
-  exact cnd₀_of_aState_tr h₃ h₄
-  
-theorem cnd₀_simulate_of_aState {s} {a : AStrat} {d : DStrat} {n}
-[hs : AState s] [ha : a.WF] [hd : d.WF] (h : cnd₀ s) :
-cnd₀ # sys.simulate (Strat.f ⟨a, edge₀.defense.st d⟩) s n |>.1 := by
-  apply sys.fst_simulate_ind _ n; clear n; intro n s' h₁
-  exact cnd₀_simulate_full_of_aState h h₁
+  have h₅ : s'.pw = s.pw
+  · apply pw_eq_of_reachable
+    exact sys.reachable_of_simulate_eq h₂
+  rw [←h₅] at hpw
+  exact aPos_y_lt_zero_of_tr_aState_cnd₀ h₄ h₃
 
-theorem edge₀_simulate_aPos_y_lt_zero_of_aState {s} {a : AStrat} {d : DStrat} {n}
+include hpw in
+theorem edge₀_simulate_aPos_y_lt_zero_of_aState {a : AStrat} {d : DStrat} {n}
 [hs : AState s] [ha : a.WF] [hd : d.WF] (h : s.aPos.y ≤ -6) :
-sys.simulate (Strat.f ⟨a, edge₀.defense.st d⟩) s n |>.1.aPos.y < 0 :=
-  aPos_y_lt_zero_of_cnd₀ # cnd₀_simulate_of_aState # cnd₀_of_aPos_y_le_neg_6 h
+sys.simulate (Strat.f ⟨a, edge₀.defense.st d⟩) s n |>.1.aPos.y < 0 := by
+  apply sys.fst_simulate_ind (p := (·.aPos.y < 0)) _ n; clear n; intro n s' h₁
+  exact edge₀_simulate_full_aPos_y_lt_zero_of_aState h h₁
 
-theorem edge₀_simulate_aPos_y_lt_zero {s} {a : AStrat} {d : DStrat} {n}
+include hpw in
+theorem edge₀_simulate_aPos_y_lt_zero {a : AStrat} {d : DStrat} {n}
 [hs : sys.WF s] [ha : a.WF] [hd : d.WF] (h : s.aPos.y ≤ -6) :
 sys.simulate (Strat.f ⟨a, edge₀.defense.st d⟩) s n |>.1.aPos.y < 0 := by
   replace hs := s.aState_or_dState
@@ -87,12 +104,14 @@ sys.simulate (Strat.f ⟨a, edge₀.defense.st d⟩) s n |>.1.aPos.y < 0 := by
   cases n; simp; linarith; nm n
   simp [System.simulate]; split; simp; linarith; nm x s₁ h₁; clear x
   have hs₁ := AState.of_tr h₁
+  rw [←pw_eq_of_tr h₁] at hpw
   apply edge₀_simulate_aPos_y_lt_zero_of_aState
   rwa [DState.aPos_eq_of_tr h₁]
 
 theorem wf_defense_edge₀ : edge₀.defense.WF := by
   use validTr_defense
   intro s hs h a ha d hd n
+  have hpw : Fact # s.pw = 1; use h.1
   simp [defense, points, memPoints]
   apply edge₀_simulate_aPos_y_lt_zero
   simp [defense, dist] at h
